upd

coqimp/ext/compositionality.v
@@ -1,4 +1,4 @@
-(*+ Compositionality +*)
+(*+ Compositionality +*)   
 Require Import Coqlib.     
 Require Import Maps.
 
@@ -25,8 +25,33 @@ Set Implicit Arguments.
 Unset Strict Implicit.
 
 Open Scope code_scope.
-Open Scope mem_scope. Print LH__.
+Open Scope mem_scope. 
 
+(** Auxiliary Lemmas about Steps *)
+Lemma star_tau_step_impl_star_step :
+  forall A P P' (step : A -> msg -> A -> Prop),
+    star_tau_step step P P' ->
+    star_step step P P'.
+Proof.
+  intros.
+  induction H.
+  econstructor; eauto.
+  eapply multi_step; eauto.
+Qed.
+
+Lemma multi_step_cons :
+  forall A P P' P'' (step : A -> msg -> A -> Prop),
+    star_step step P P' -> star_step step P' P'' ->
+    star_step step P P''.
+Proof.
+  intros.
+  generalize dependent P.
+  induction H0; intros; eauto.
+  eapply IHstar_step in H1; eauto.
+  eapply multi_step; eauto.
+Qed.
+
+(** Define Well-formed Current Thread and Well-formed Ready *)
 Inductive wfIndex : XCodeHeap -> State -> Word -> Index -> Prop :=
 | cons_wfIndex : forall C M R F D idx pc,
     (
@@ -55,11 +80,11 @@ Inductive wfHPrimExec : XCodeHeap -> primcom -> HState -> Prop :=
     wfHPrimExec C A HS.
 
 (** Well-formed Current Thread *)
-Inductive wfCth : Index -> LProg -> HProg -> Prop :=
+Inductive wfCth : Index -> XCodeHeap * XCodeHeap -> LProg -> HProg -> Prop :=
 | clt_wfCth : forall C Cas S HS pc npc PrimSet idx,
-    indom pc C -> wp_stateRel S HS -> wfIndex C S pc idx -> 
+    wp_stateRel S HS -> wfIndex C S pc idx -> 
     get_Hs_pcont HS = (pc, npc) ->
-    wfCth idx (C ⊎ Cas, (S, pc, npc)) (C, PrimSet, HS)
+    wfCth idx (C, Cas) (C ⊎ Cas, (S, pc, npc)) (C, PrimSet, HS)
 
 | prim_wfCth : forall C Cas Sc HSc S HS Sr HSr w Q Pr A pc npc PrimSet idx k,
     state_union Sc Sr S -> hstate_union HSc HSr HS ->
@@ -67,31 +92,272 @@ Inductive wfCth : Index -> LProg -> HProg -> Prop :=
     (
       forall S' HS' w' f, (S', HS', Pdone, w') ||= Q ⋆ Pr -> getregs S' r15 = Some (W f) ->
                           HProgSafe (C, PrimSet, HS') ->
-                        exists idx_j, wfCth idx_j (C ⊎ Cas, (S', f +ᵢ ($ 8), f +ᵢ ($ 12))) (C, PrimSet, HS')
+                        exists idx_j, wfCth idx_j (C, Cas) (C ⊎ Cas, (S', f +ᵢ ($ 8), f +ᵢ ($ 12))) (C, PrimSet, HS')
     ) ->
-    wfCth idx (C ⊎ Cas, (S, pc, npc)) (C, PrimSet, HS).
+    wfCth idx (C, Cas) (C ⊎ Cas, (S, pc, npc)) (C, PrimSet, HS).
 
 (* Well-formed Ready Thread *)
-Inductive wfRdy : XCodeHeap -> XCodeHeap * apSet -> Tid -> tlocst -> Prop :=
-| cons_wfRdy : forall S HS t K PrimSet C C',
+Inductive wfRdy : XCodeHeap * XCodeHeap -> XCodeHeap * apSet -> Tid -> tlocst -> Prop :=
+| cons_wfRdy : forall t K PrimSet C Cas,
     (
-      forall f T HM pc npc, 
+      forall S HS f T HM pc npc, 
         wp_stateRel S HS -> HS = (T, t, K, HM) -> HProgSafe (C, PrimSet, HS) ->
         getregs S r15 = Some (W f) -> pc = f +ᵢ ($ 8) -> npc = f +ᵢ ($ 12) ->
-        exists idx, wfCth idx (C, (S, pc, npc)) (C, PrimSet, HS)
+        get_Hs_pcont HS = (pc, npc) ->
+        exists idx, wfCth idx (C, Cas) (C ⊎ Cas, (S, pc, npc)) (C, PrimSet, HS)
     ) ->
-    wfRdy C (C', PrimSet) t K.
+    wfRdy (C, Cas) (C, PrimSet) t K.
+
+Lemma indom_get_left :
+  forall tp tp' (M M' : tp -> option tp') l v,
+    (M ⊎ M') l = v -> indom l M ->
+    M l = v.
+Proof.
+  intros.
+  unfold merge in *.
+  destruct (M l) eqn:Heq; eauto.
+  unfold indom in *.
+  destruct H0; tryfalse.
+Qed.
+
+Lemma LP__local1 :
+  forall S S' pc npc pc' npc' C C' m,
+    indom pc C ->
+    LP__ (C ⊎ C', (S, pc, npc)) m (C ⊎ C', (S', pc', npc')) ->
+    LP__ (C, (S, pc, npc)) m (C, (S', pc', npc')).
+Proof.
+  intros.
+  inv H0.
+  inv H10.
+  econstructor; eauto.
+  eapply LNTrans; eauto.
+  eapply indom_get_left; eauto.
+  econstructor; eauto.
+  eapply LJumpl; eauto.
+  eapply indom_get_left; eauto.
+  econstructor; eauto.
+  eapply LCall; eauto.
+  eapply indom_get_left; eauto.
+  econstructor; eauto.
+  eapply LRetl; eauto.
+  eapply indom_get_left; eauto.
+  econstructor; eauto.
+  eapply LBe_true; eauto.
+  eapply indom_get_left; eauto.
+  econstructor; eauto.
+  eapply LBe_false; eauto.
+  eapply indom_get_left; eauto.
+  econstructor; eauto.
+  eapply LPrint; eauto.
+  eapply indom_get_left; eauto.
+  econstructor; eauto.
+  eapply LPsave_no_trap; eauto.
+  eapply indom_get_left; eauto.
+  econstructor; eauto.
+  eapply LPsave_trap; eauto.
+  eapply indom_get_left; eauto.
+  econstructor; eauto.
+  eapply LPrestore_no_trap; eauto.
+  eapply indom_get_left; eauto.
+  econstructor; eauto.
+  eapply LPrestore_trap; eauto.
+  eapply indom_get_left; eauto.
+Qed.
+
+Lemma LH__progress_HH__progress :
+  forall C Mc Mr LR F pc npc LM' LR' F' D' pc' npc' T t HR b HF M PrimSet,
+    LH__ C ((Mc ⊎ Mr ⊎ M, (LR, F), []), pc, npc) tau
+         ((LM', (LR', F'), D'), pc', npc') ->
+    HProgSafe (C, PrimSet, (T, t, ((HR, b, HF), pc, npc), M)) ->
+    indom pc C -> Mc ⊥ Mr -> (Mc ⊎ Mr) ⊥ M ->
+    curTRel (Mc, (LR, F)) (t, ((HR, b, HF), pc, npc)) ->
+    exists Mc' M' K',
+      LM' = Mc' ⊎ Mr ⊎ M' /\ Mc' ⊥ Mr -> (Mc' ⊎ Mr) ⊥ M'
+      /\ HP__ (C, PrimSet, (T, t, ((HR, b, HF), pc, npc), M)) tau (C, PrimSet, (T, t, K', M'))
+      /\ curTRel (Mc', (LR', F')) (t, K') /\ D' = nil.
+Proof.
+Admitted.
+
+(* WfCth and WfRdy Preservation *)
+Lemma wfCth_wfRdy_tau_step_preservation :
+  forall idx C Cas S pc npc S' pc' npc' PrimSet T t K M Spec,
+    simImpsPrimSet Spec Cas PrimSet -> C ⊥ Cas -> 
+    HProgSafe (C, PrimSet, (T, t, K, M)) ->
+    wfCth idx (C, Cas) (C ⊎ Cas, (S, pc, npc)) (C, PrimSet, (T, t, K, M)) ->
+    (
+      forall t' K', (ThrdMap.set t None T) t' = Some K' ->
+                    wfRdy (C, Cas) (C, PrimSet) t' K' 
+    ) ->
+    LP__ (C ⊎ Cas, (S, pc, npc)) tau (C ⊎ Cas, (S', pc', npc')) ->
+    exists T' t0 K0 M' idx1,
+      ((idx1 ⩹ idx /\ (T, t, K, M) = (T', t0, K0, M')) \/
+       (exists HP', star_tau_step HP__ (C, PrimSet, (T, t, K, M)) HP' /\
+                    HP__ HP' tau (C, PrimSet, (T', t0, K0, M'))))
+      /\
+      wfCth idx1 (C, Cas) (C ⊎ Cas, (S', pc', npc')) (C, PrimSet, (T', t0, K0, M')) /\
+      (
+        forall t1 K1, (ThrdMap.set t0 None T') t1 = Some K1 ->
+                      wfRdy (C, Cas) (C, PrimSet) t1 K1 
+      ).
+Proof.
+  intros.
+  lets Ht : classic (indom pc C).
+  destruct Ht as [Ht | Ht].
+  {  
+    inv H2.
+    {
+      inv H10.
+      eapply LP__local1 in H4; eauto.
+      inv H4.
+      simpl in H18.
+      destruct K.
+      destruct p.
+      destruct h.
+      destruct p.
+      renames h0 to HR, z to b, h to HF.
+      simpl in H15.
+      inv H15.
+      inv H18.
+
+      assert ((Mc ⊎ MT) ⊎ MemMap.set TaskCur (Some (Ptr (t, $ 0))) empM =
+              Mc ⊎ (MT ⊎ MemMap.set TaskCur (Some (Ptr (t, $ 0))) empM)).
+      {
+        rewrite <- lemmas.merge_assoc; eauto.
+      }
+             
+      assert (((Mc ⊎ MT) ⊎ MemMap.set TaskCur (Some (Ptr (t, $ 0))) empM) ⊎ M =
+              Mc ⊎ (MT ⊎ MemMap.set TaskCur (Some (Ptr (t, $ 0))) empM) ⊎ M).
+      {
+        rewrite H2; eauto.
+      }
+
+      assert (Mc ⊥ (MT ⊎ MemMap.set TaskCur (Some (Ptr (t, $ 0))) empM)).
+      {
+        eapply lemmas.disj_sep_merge_still; eauto.
+      }
+      
+      unfold Tid in H4.
+      rewrite H4 in H22.
+      eapply LH__progress_HH__progress in H22; eauto.
+    }
+  }
+Admitted.
+
+Lemma wfCth_wfRdy_event_step_preservation :
+  forall idx C Cas S pc npc S' pc' npc' PrimSet T t K M Spec v,
+    simImpsPrimSet Spec Cas PrimSet -> C ⊥ Cas -> 
+    HProgSafe (C, PrimSet, (T, t, K, M)) ->
+    wfCth idx (C, Cas) (C ⊎ Cas, (S, pc, npc)) (C, PrimSet, (T, t, K, M)) ->
+    (
+      forall t' K', (ThrdMap.set t None T) t' = Some K' ->
+                    wfRdy (C, Cas) (C, PrimSet) t' K' 
+    ) ->
+    LP__ (C ⊎ Cas, (S, pc, npc)) (out v) (C ⊎ Cas, (S', pc', npc')) ->
+    exists T' t0 K0 M' idx1 HP',
+      (
+        star_tau_step HP__ (C, PrimSet, (T, t, K, M)) HP' /\
+                    HP__ HP' (out v) (C, PrimSet, (T', t0, K0, M'))
+      )
+      /\
+      wfCth idx1 (C, Cas) (C ⊎ Cas, (S', pc', npc')) (C, PrimSet, (T', t0, K0, M')) /\
+      (
+        forall t1 K1, (ThrdMap.set t0 None T') t1 = Some K1 ->
+                      wfRdy (C, Cas) (C, PrimSet) t1 K1 
+      ).
+Proof.
+Admitted.
+
+Lemma wfCth_wfRdy_abort_preservation :
+  forall idx C Cas S pc npc PrimSet T t K M Spec m,
+    simImpsPrimSet Spec Cas PrimSet -> C ⊥ Cas -> 
+    HProgSafe (C, PrimSet, (T, t, K, M)) ->
+    wfCth idx (C, Cas) (C ⊎ Cas, (S, pc, npc)) (C, PrimSet, (T, t, K, M)) ->
+    (
+      forall t' K', (ThrdMap.set t None T) t' = Some K' ->
+                    wfRdy (C, Cas) (C, PrimSet) t' K' 
+    ) ->
+    ~ (exists LP' : LProg, LP__ (C ⊎ Cas, (S, pc, npc)) m LP') ->
+    exists HP' : HProg, star_tau_step HP__ (C, PrimSet, (T, t, K, M)) HP' /\ ~ (exists (HP'': HProg) m', HP__ HP' m' HP'').
+Proof.
+Admitted.
 
 (* Compositionality Proof *)
 Lemma wfCth_wfRdy_imply_wpsim :
   forall idx C Cas S pc npc PrimSet T t K M Spec,
     simImpsPrimSet Spec Cas PrimSet -> C ⊥ Cas -> 
     HProgSafe (C, PrimSet, (T, t, K, M)) ->
-    wfCth idx (C ⊎ Cas, (S, pc, npc)) (C, PrimSet, (T, t, K, M)) ->
+    wfCth idx (C, Cas) (C ⊎ Cas, (S, pc, npc)) (C, PrimSet, (T, t, K, M)) ->
     (
       forall t' K', (ThrdMap.set t None T) t' = Some K' ->
-                    wfRdy (C ⊎ Cas) (C, PrimSet) t' K' 
+                    wfRdy (C, Cas) (C, PrimSet) t' K' 
     ) ->
     wp_sim idx (C ⊎ Cas, (S, pc, npc)) (C, PrimSet, (T, t, K, M)).
 Proof.
-Admitted.
+  cofix Hp; intros.
+  econstructor; intros.
+  {
+    (* tau *)
+    lets Hpreserve : H2.
+    lets HLP : H4.
+    inv H4.
+    eapply wfCth_wfRdy_tau_step_preservation in Hpreserve; eauto.
+    destruct Hpreserve as (T' & t0 & K0 & M' & idx1 & Hpreserve).
+    destruct Hpreserve as (Hstep & HwfCth & HwfRdy).
+    destruct Hstep as [ (Hlt & Hno_step) | (HP' & HHstar_step & HHstep) ].
+    {
+      left.
+      exists idx1.
+      split; eauto.
+      inv Hno_step.
+      eapply Hp; eauto.
+    }
+    {
+      right.
+      exists idx1 HP' (C, PrimSet, (T', t0, K0, M')).
+      split; eauto.
+      split; eauto.
+      eapply Hp; eauto.
+      clear - H1 HHstar_step HHstep.
+      unfolds HProgSafe.
+      intros.
+      assert (star_tau_step HP__ (C, PrimSet, (T, t, K, M)) (C, PrimSet, (T', t0, K0, M'))).
+      econstructor; eauto.
+      eapply star_tau_step_impl_star_step in H0.
+      assert (Hstar : star_step HP__ (C, PrimSet, (T, t, K, M)) hp').
+      eapply multi_step_cons; eauto.
+      eapply H1 in Hstar; eauto.
+    }
+  }
+  {
+    (* event *)
+    lets Hpreserve : H2.
+    lets HLP : H4.
+    inv H4.    
+    eapply wfCth_wfRdy_event_step_preservation in Hpreserve; eauto. 
+    destruct Hpreserve as (T' & t0 & K0 & M' & idx1 & HP' & (HH_star_steps & HHstep)
+                           & HwfCth & Hwfrdy).
+    do 3 eexists.
+    split; eauto.
+    split; eauto.
+    instantiate (1 := idx1).
+    eapply Hp; eauto.
+    clear - H1 HH_star_steps HHstep.
+    unfolds HProgSafe; intros.
+    eapply star_tau_step_impl_star_step in HH_star_steps.
+    assert (star_step HP__ (C, PrimSet, (T, t, K, M)) (C, PrimSet, (T', t0, K0, M'))).
+    eapply multi_step; eauto.
+    assert (Hstar : star_step HP__ (C, PrimSet, (T, t, K, M)) hp').
+    eapply multi_step_cons; eauto.
+    eapply H1 in Hstar; eauto.
+  }
+  {
+    (* abort *)
+    eapply wfCth_wfRdy_abort_preservation in H4; eauto.
+    destruct H4 as (HP' & HHstar_steps & HHstep).
+    clear - H1 HHstar_steps HHstep.
+    unfolds HProgSafe.
+    eapply star_tau_step_impl_star_step in HHstar_steps.
+    eapply H1 in HHstar_steps.
+    tryfalse.
+  }
+Qed.
